src/Init/Data/Array/BasicAux.lean
@@ -32,11 +32,6 @@ private theorem List.of_toArrayAux_eq_toArrayAux {as bs : List α} {cs ds : Arra
     have := Array.of_push_eq_push ih₂
     simp [this]
 
-@[simp] theorem List.toArray_eq_toArray_eq (as bs : List α) : (as.toArray = bs.toArray) = (as = bs) := by
-  apply propext; apply Iff.intro
-  · intro h; simp [toArray] at h; have := of_toArrayAux_eq_toArrayAux h rfl; exact this.1
-  · intro h; rw [h]
-
 def Array.mapM' [Monad m] (f : α → m β) (as : Array α) : m { bs : Array β // bs.size = as.size } :=
   go 0 ⟨mkEmpty as.size, rfl⟩ (by simp_arith)
 where
