tests/lean/csimpAttrToArray.lean
@@ -1,0 +1,3 @@
+set_option trace.compiler.ir.init true
+def f (as : List Nat) : Array Nat :=
+  as.toArray
